iris_heap_lang/class_instances.v
@@ -50,6 +50,8 @@ Section atomic.
   Proof. solve_atomic. Qed.
   Global Instance load_atomic s v : Atomic s (Load (Val v)).
   Proof. solve_atomic. Qed.
+  Global Instance xchg_atomic s v1 v2 : Atomic s (Xchg (Val v1) (Val v2)).
+  Proof. solve_atomic. Qed.
   Global Instance store_atomic s v1 v2 : Atomic s (Store (Val v1) (Val v2)).
   Proof. solve_atomic. Qed.
   Global Instance cmpxchg_atomic s v0 v1 v2 : Atomic s (CmpXchg (Val v0) (Val v1) (Val v2)).
